Semantics/TreeToGraphThms.thy
@@ -137,6 +137,12 @@ lemma rep_integer_less_than [rep]:
    (\<exists>xe ye. e = BinaryExpr BinIntegerLessThan xe ye)"
   by (induction rule: rep.induct; auto)
 
+lemma rep_integer_mul_high [rep]:
+  "g \<turnstile> n \<simeq> e \<Longrightarrow>
+   kind g n = IntegerMulHighNode x y \<Longrightarrow>
+   (\<exists>xe ye. e = BinaryExpr BinIntegerMulHigh xe ye)"
+  by (induction rule: rep.induct; auto)
+
 lemma rep_integer_test [rep]:
   "g \<turnstile> n \<simeq> e \<Longrightarrow>
    kind g n = IntegerTestNode x y \<Longrightarrow>
@@ -238,11 +244,11 @@ proof (induction arbitrary: e\<^sub>2 rule: "rep.induct")
 next
   case (ParameterNode n i s)
   then show ?case
-    by (metis IRNode.distinct(2851,2885) ParameterNodeE rep_parameter)
+    by (metis IRNode.distinct(2965,2999) ParameterNodeE rep_parameter)
 next
   case (ConditionalNode n c t f ce te fe)
   then show ?case
-    by (metis IRNode.distinct(607,641) IRNode.inject(6) ConditionalNodeE rep_conditional)
+    by (metis IRNode.distinct(619,653) IRNode.inject(6) ConditionalNodeE rep_conditional)
 next
   case (AbsNode n x xe)
   then show ?case
@@ -314,28 +320,31 @@ next
 next
   case (IntegerTestNode n x y xe ye)
   then show ?case
-    by (metis IRNode.distinct(1751,1785) IRNode.inject(18) IntegerTestNodeE rep_integer_test)
+    by (solve_det node: IntegerTestNode)
 next
   case (IntegerNormalizeCompareNode n x y xe ye)
   then show ?case
-    by (metis (no_types, lifting) IntegerNormalizeCompareNodeE rep_integer_normalize_compare
-        IRNode.distinct(1675,1709) IRNode.inject(17))
+    by (solve_det node: IntegerNormalizeCompareNode)
+next
+  case (IntegerMulHighNode n x xe)
+  then show ?case
+    by (solve_det node: IntegerMulHighNode)
 next
   case (NarrowNode n x xe)
   then show ?case
-    by (metis IRNode.distinct(2605,2639) IRNode.inject(32) NarrowNodeE rep_narrow)
+    by (metis IRNode.distinct(2719,2753) IRNode.inject(33) NarrowNodeE rep_narrow)
 next
   case (SignExtendNode n x xe)
   then show ?case
-    by (metis IRNode.distinct(2893,3035) IRNode.inject(43) SignExtendNodeE rep_sign_extend)
+    by (metis IRNode.distinct(3007,3149) IRNode.inject(44) SignExtendNodeE rep_sign_extend)
 next
   case (ZeroExtendNode n x xe)
   then show ?case
-    by (metis IRNode.distinct(2915,3189) IRNode.inject(54) ZeroExtendNodeE rep_zero_extend)
+    by (metis IRNode.distinct(3029,3303) IRNode.inject(55) ZeroExtendNodeE rep_zero_extend)
 next
   case (LeafNode n s)
   then show ?case
-    by (metis is_preevaluated.simps(43,57) rep_load_field LeafNodeE)
+    by (metis is_preevaluated.simps(44,58) rep_load_field LeafNodeE)
 next
   case (RefNode n')
   then show ?case
@@ -347,7 +356,7 @@ next
 next
   case (IsNullNode n v)
   then show ?case
-    by (metis IRNode.distinct(1967,2001) IRNode.inject(21) IsNullNodeE rep_is_null)
+    by (metis IRNode.distinct(2081,2115) IRNode.inject(22) IsNullNodeE rep_is_null)
 qed
 
 lemma repAllDet:
@@ -1076,9 +1085,9 @@ BinaryExpr BinIntegerLessThan xe1 ye1 \<ge> BinaryExpr BinIntegerLessThan xe2 ye
       obtain xn yn where l: "kind g1 n = IntegerTestNode xn yn"
         by (simp add: IntegerTestNode.hyps(1))
       then have mx: "g1 \<turnstile> xn \<simeq> xe1"
-        using IRNode.inject(18) IntegerTestNode.hyps(1,2) by presburger
+        using IRNode.inject(19) IntegerTestNode.hyps(1,2) by presburger
       from l have my: "g1 \<turnstile> yn \<simeq> ye1"
-        by (metis IRNode.inject(18) IntegerTestNode.hyps(1,3))
+        by (metis IRNode.inject(19) IntegerTestNode.hyps(1,3))
       then show ?case
       proof -
         have "g1 \<turnstile> xn \<simeq> xe1"
@@ -1087,10 +1096,10 @@ BinaryExpr BinIntegerLessThan xe1 ye1 \<ge> BinaryExpr BinIntegerLessThan xe2 ye
           by (simp add: my)
         have xer: "\<exists> xe2. (g2 \<turnstile> xn \<simeq> xe2) \<and> xe1 \<ge> xe2"
           using IntegerTestNode a b c d l no_encoding not_excluded_keep_type repDet singletonD
-          by (metis IRNode.inject(18))
+          by (metis IRNode.inject(19))
         have "\<exists> ye2. (g2 \<turnstile> yn \<simeq> ye2) \<and> ye1 \<ge> ye2"
           using IntegerLessThanNode a b c d l no_encoding not_excluded_keep_type repDet singletonD
-          by (metis IRNode.inject(18) IntegerTestNode.IH(2) IntegerTestNode.hyps(1) my)
+          by (metis IRNode.inject(19) IntegerTestNode.IH(2) IntegerTestNode.hyps(1) my)
         then have "\<exists> xe2 ye2. (g2 \<turnstile> n \<simeq> BinaryExpr BinIntegerTest xe2 ye2) \<and> 
     BinaryExpr BinIntegerTest xe1 ye1 \<ge> BinaryExpr BinIntegerTest xe2 ye2"
           by (metis IntegerTestNode.prems l mono_binary xer rep.IntegerTestNode)
@@ -1104,9 +1113,9 @@ BinaryExpr BinIntegerLessThan xe1 ye1 \<ge> BinaryExpr BinIntegerLessThan xe2 ye
       obtain xn yn where l: "kind g1 n = IntegerNormalizeCompareNode xn yn"
         by (simp add: IntegerNormalizeCompareNode.hyps(1))
       then have mx: "g1 \<turnstile> xn \<simeq> xe1"
-        using IRNode.inject(17) IntegerNormalizeCompareNode.hyps(1,2) by presburger
+        using IRNode.inject(18) IntegerNormalizeCompareNode.hyps(1,2) by presburger
       from l have my: "g1 \<turnstile> yn \<simeq> ye1"
-        using IRNode.inject(17) IntegerNormalizeCompareNode.hyps(1,3) by presburger
+        using IRNode.inject(18) IntegerNormalizeCompareNode.hyps(1,3) by presburger
       then show ?case
       proof -
         have "g1 \<turnstile> xn \<simeq> xe1"
@@ -1114,15 +1123,43 @@ BinaryExpr BinIntegerLessThan xe1 ye1 \<ge> BinaryExpr BinIntegerLessThan xe2 ye
         have "g1 \<turnstile> yn \<simeq> ye1"
           by (simp add: my)
         have xer: "\<exists> xe2. (g2 \<turnstile> xn \<simeq> xe2) \<and> xe1 \<ge> xe2"
-          by (metis IRNode.inject(17) IntegerNormalizeCompareNode.IH(1) l mx no_encoding a b c d
+          by (metis IRNode.inject(18) IntegerNormalizeCompareNode.IH(1) l mx no_encoding a b c d
               IntegerNormalizeCompareNode.hyps(1) emptyE insertE not_excluded_keep_type repDet)
         have "\<exists> ye2. (g2 \<turnstile> yn \<simeq> ye2) \<and> ye1 \<ge> ye2"
-          by (metis IRNode.inject(17) IntegerNormalizeCompareNode.IH(2) my no_encoding a b c d l
+          by (metis IRNode.inject(18) IntegerNormalizeCompareNode.IH(2) my no_encoding a b c d l
               IntegerNormalizeCompareNode.hyps(1) emptyE insertE not_excluded_keep_type repDet)
         then have "\<exists> xe2 ye2. (g2 \<turnstile> n \<simeq> BinaryExpr BinIntegerNormalizeCompare xe2 ye2) \<and>
     BinaryExpr BinIntegerNormalizeCompare xe1 ye1 \<ge> BinaryExpr BinIntegerNormalizeCompare xe2 ye2"
           by (metis IntegerNormalizeCompareNode.prems l mono_binary rep.IntegerNormalizeCompareNode
               xer)
+        then show ?thesis
+          by meson
+      qed
+    next
+      case (IntegerMulHighNode n x y xe1 ye1)
+      have k: "g1 \<turnstile> n \<simeq> BinaryExpr BinIntegerMulHigh xe1 ye1"
+        by (simp add: IntegerMulHighNode.hyps(1,2,3) rep.IntegerMulHighNode)
+      obtain xn yn where l: "kind g1 n = IntegerMulHighNode xn yn"
+        by (simp add: IntegerMulHighNode.hyps(1))
+      then have mx: "g1 \<turnstile> xn \<simeq> xe1"
+        using IRNode.inject(17) IntegerMulHighNode.hyps(1,2) by presburger
+      from l have my: "g1 \<turnstile> yn \<simeq> ye1"
+        using IRNode.inject(17) IntegerMulHighNode.hyps(1,3) by presburger
+      then show ?case
+      proof -
+        have "g1 \<turnstile> xn \<simeq> xe1"
+          by (simp add: mx)
+        have "g1 \<turnstile> yn \<simeq> ye1"
+          by (simp add: my)
+        have xer: "\<exists> xe2. (g2 \<turnstile> xn \<simeq> xe2) \<and> xe1 \<ge> xe2"
+          by (metis IRNode.inject(17) IntegerMulHighNode.IH(1) IntegerMulHighNode.hyps(1) a b c d
+              emptyE insertE l mx no_encoding not_excluded_keep_type repDet)
+        have "\<exists> ye2. (g2 \<turnstile> yn \<simeq> ye2) \<and> ye1 \<ge> ye2"
+          by (metis IRNode.inject(17) IntegerMulHighNode.IH(2) IntegerMulHighNode.hyps(1) a b c d
+              emptyE insertE l my no_encoding not_excluded_keep_type repDet)
+        then have "\<exists> xe2 ye2. (g2 \<turnstile> n \<simeq> BinaryExpr BinIntegerMulHigh xe2 ye2) \<and>
+ BinaryExpr BinIntegerMulHigh xe1 ye1 \<ge> BinaryExpr BinIntegerMulHigh xe2 ye2"
+          by (metis IntegerMulHighNode.prems l mono_binary rep.IntegerMulHighNode xer)
         then show ?thesis
           by meson
       qed
@@ -1339,6 +1376,7 @@ lemma subset_implies_evals:
        apply (solve_subset_eval as_set: assms(1) eval: IntegerLessThanNode)
        apply (solve_subset_eval as_set: assms(1) eval: IntegerTestNode)
       apply (solve_subset_eval as_set: assms(1) eval: IntegerNormalizeCompareNode)
+      apply (solve_subset_eval as_set: assms(1) eval: IntegerMulHighNode)
       apply (solve_subset_eval as_set: assms(1) eval: NarrowNode)
      apply (solve_subset_eval as_set: assms(1) eval: SignExtendNode)
     apply (solve_subset_eval as_set: assms(1) eval: ZeroExtendNode)
@@ -1446,6 +1484,7 @@ lemma graph_unchanged_rep_unchanged:
          apply (metis no_encoding rep.IntegerLessThanNode)
          apply (metis no_encoding rep.IntegerTestNode)
         apply (metis no_encoding rep.IntegerNormalizeCompareNode)
+        apply (metis no_encoding rep.IntegerMulHighNode)
         apply (metis no_encoding rep.NarrowNode)
        apply (metis no_encoding rep.SignExtendNode)
       apply (metis no_encoding rep.ZeroExtendNode)
@@ -1553,7 +1592,7 @@ theorem term_graph_reconstruction:
   next
     case (ParameterNodeNew g i s)
     then show ?case
-      by (metis IRNode.distinct(2883) ParameterNode find_new_kind find_new_stamp)
+      by (metis IRNode.distinct(2997) ParameterNode find_new_kind find_new_stamp)
   next
     case (ConditionalNodeSame g4 c t f s' n g ce g2 te g3 fe)
     then have k: "kind g4 n = ConditionalNode c t f"
@@ -1622,10 +1661,10 @@ theorem term_graph_reconstruction:
       by (simp add: local.BinaryNodeSame)
     then show ?case 
       using x k apply (cases op)
-      using bin_node.simps(1,2,3,4,5,6,7,8,9,10,11,12,13,14,15)
+      using bin_node.simps(1,2,3,4,5,6,7,8,9,10,11,12,13,14,15,16)
             AddNode MulNode SubNode AndNode OrNode ShortCircuitOrNode LeftShiftNode RightShiftNode 
             UnsignedRightShiftNode IntegerEqualsNode IntegerLessThanNode IntegerBelowNode XorNode
-            IntegerTestNode IntegerNormalizeCompareNode
+            IntegerTestNode IntegerNormalizeCompareNode IntegerMulHighNode
       by presburger+
   next
     case (BinaryNodeNew g3 op x y s' g xe g2 ye n g')
@@ -1643,10 +1682,10 @@ theorem term_graph_reconstruction:
       by (meson fresh_node_preserves_other_nodes no_encoding)
     then show ?case 
       using x k apply (cases op)
-      using bin_node.simps(1,2,3,4,5,6,7,8,9,10,11,12,13,14,15)
+      using bin_node.simps(1,2,3,4,5,6,7,8,9,10,11,12,13,14,15,16)
             AddNode MulNode SubNode AndNode OrNode ShortCircuitOrNode LeftShiftNode RightShiftNode
             UnsignedRightShiftNode IntegerEqualsNode IntegerLessThanNode XorNode IntegerBelowNode
-            IntegerTestNode IntegerNormalizeCompareNode
+            IntegerTestNode IntegerNormalizeCompareNode IntegerMulHighNode
       by presburger+
   next
     case (AllLeafNodes g n s)
@@ -2049,6 +2088,7 @@ lemma same_kind_stamp_encodes_equal:
          apply (metis IntegerLessThanNode)
           apply (metis IntegerTestNode)
         apply (metis IntegerNormalizeCompareNode)
+        apply (metis IntegerMulHighNode)
         apply (metis NarrowNode)
        apply (metis SignExtendNode)
       apply (metis ZeroExtendNode)
@@ -2461,6 +2501,20 @@ next
       using IntegerNormalizeCompareNode.IH(1,2) kind kind_eq rep.IntegerNormalizeCompareNode
             stamp_eq by blast
   next
+    case (IntegerMulHighNode n x y xe ye)
+    then have kind: "kind g n = IntegerMulHighNode x y"
+      by simp
+    then have isin: "n \<in> ids g"
+      by simp
+    have inputs: "{x, y} = inputs g n"
+      by (simp add: kind)
+    have "x \<in> ids g \<and> y \<in> ids g"
+      using closed wf_closed_def isin inputs by blast
+    then have "x \<notin> new \<and> y \<notin> new"
+      using unchanged by (simp add: new_def)
+    then show ?case
+      using IntegerMulHighNode.IH(1,2) kind kind_eq rep.IntegerMulHighNode stamp_eq by blast
+  next
     case (NarrowNode n inputBits resultBits x xe)
     then have kind: "kind g n = NarrowNode inputBits resultBits x"
       by simp
@@ -2706,7 +2760,7 @@ lemma unrep_preserves_closure:
   next
     case (ConstantNodeNew g c n g')
     then have dom: "ids g' = ids g \<union> {n}"
-      by (meson IRNode.distinct(739) add_node_ids_subset ids_add_update)
+      by (meson IRNode.distinct(753) add_node_ids_subset ids_add_update)
     have k: "kind g' n = ConstantNode c"
       by (simp add: add_node_lookup ConstantNodeNew)
     then have inp: "{} = inputs g' n"
@@ -2726,7 +2780,7 @@ lemma unrep_preserves_closure:
   next
     case (ParameterNodeNew g i s n g')
     then have dom: "ids g' = ids g \<union> {n}"
-      by (meson IRNode.distinct(2883) add_node_ids_subset ids_add_update)
+      by (meson IRNode.distinct(2997) add_node_ids_subset ids_add_update)
     have k: "kind g' n = ParameterNode i"
       by (simp add: add_node_lookup ParameterNodeNew)
     then have inp: "{} = inputs g' n"
@@ -2746,7 +2800,7 @@ lemma unrep_preserves_closure:
   next
     case (ConditionalNodeNew g4 c t f s' g ce g2 te g3 fe n g')
     then have dom: "ids g' = ids g4 \<union> {n}"
-      by (meson IRNode.distinct(639) add_node_ids_subset ids_add_update)
+      by (meson IRNode.distinct(651) add_node_ids_subset ids_add_update)
     have k: "kind g' n = ConditionalNode c t f"
       by (auto simp add: find_new_kind ConditionalNodeNew.hyps(10))
     then have inp: "{c, t, f} = inputs g' n"
@@ -2754,7 +2808,7 @@ lemma unrep_preserves_closure:
     from k have suc: "{} = succ g' n"
       by simp
     have "inputs g' n \<subseteq> ids g' \<and> succ g' n \<subseteq> ids g' \<and> kind g' n \<noteq> NoNode"
-      by (metis (mono_tags, lifting) ConditionalNodeNew.hyps(2,4,6) IRNode.distinct(639) insertCI k
+      by (metis (mono_tags, lifting) ConditionalNodeNew.hyps(2,4,6) IRNode.distinct(651) insertCI k
           Un_empty_right Un_insert_right dom empty_subsetI in_mono insert_subsetI unrep_contains
           unrep_ids_subset inp suc)
     then show ?case 
